Hacks

proof/Simple/SubstValueValue.v
@@ -4,32 +4,71 @@ Require Export Exp.
 
 
 (** Substitution ****************************************************)
-Fixpoint liftX (n: nat) (depth: nat) (xx: exp) : exp :=
- match xx with 
- | XVar ix    => if bge_nat ix depth
-                  then XVar (ix + n)
-                  else xx
 
- | XLam t1 x1 => XLam t1 (liftX n (S depth) x1)
+(* When we push new elements on the environment stack of an
+   expression, we need to lift free indices in the expression 
+   across the new elements.
 
- | XApp x1 x2 => XApp (liftX n depth x1)
-                      (liftX n depth x2)
- end.
+   For example given: 
+             t1, t0 |- 0 1 (\. 0 1 2) :: t3
+
+   Pushing two more elements gives:
+     t1, t0, ta, tb |- 2 3 (\. 0 3 4) :: t3
+ *)
+Fixpoint 
+ liftX  (n:  nat) (* number of new elements pushed on environment *)
+        (d:  nat) (* current binding depth in expression *)
+        (xx: exp) (* expression to lift *)
+        : exp
+ := match xx with 
+    |  XVar ix    
+    => if bge_nat ix d
+        (* var was pointing into env, lift it across new elems *)
+        then XVar (ix + n)
+        (* var was locally bound, leave it be *)
+        else xx
+
+    (* increase the depth as we move across a lambda *)
+    |  XLam t1 x1
+    => XLam t1 (liftX n (S d) x1)
+
+    |  XApp x1 x2
+    => XApp   (liftX n d x1) (liftX n d x2)
+    end.
 
 
-Fixpoint subst' (depth: nat) (u: exp) (xx: exp)  : exp :=
- match xx with
- | XVar ix    =>  match compare ix depth with
-                  | EQ => liftX depth 0 u
-                  | GT => XVar (ix - 1)
-                  | _  => XVar ix
-                  end
+(* Substitute for the outermost binder in an expression. *)
+Fixpoint
+ subst' (d:  nat) (* current binding depth in expression *)
+        (u:  exp) (* new expression to substitute *)
+        (xx: exp) (* expression to substitute into *)
+        : exp 
+ := match xx with
+    | XVar ix 
+    => match compare ix d with
+       (* Index matches the one we are substituting for. 
+          When we substitute the new expression, we need to lift
+          its free indices across the lambdas that we've crossed
+          to get to this point *)
+       | EQ => liftX d 0 u
+       
+       (* Index was free in the original expression.
+          As we've removed the outermost binder, also decrease this
+          index by one. *)
+       | GT => XVar (ix - 1)
 
- | XLam t1 x2 => XLam t1 (subst' (S depth) u x2)
+       (* Index was bound in the original expression. *)
+       | LT  => XVar ix
+       end
 
- | XApp x1 x2 => XApp (subst' depth u x1)
-                      (subst' depth u x2)
+    (* increase the depth as we move across a lambda *)
+    |  XLam t1 x2
+    => XLam t1 (subst' (S d) u x2)
+
+    |  XApp x1 x2 
+    => XApp (subst' d u x1) (subst' d u x2)
  end. 
+
 
 Definition  subst := subst' 0.
 Hint Unfold subst.
@@ -37,7 +76,8 @@ Hint Unfold subst.
 
 (** Lemmas **********************************************************)
 
-(* Lifting an expression by 0 steps doesn't do anything *)
+(* Lifting an expression by 0 steps doesn't do anything.
+   This is equivalent to pushing 0 things on the environment. *)
 Theorem liftX_none
  : forall x1 depth
  , liftX 0 depth x1 = x1.
@@ -56,16 +96,20 @@ Proof.
 Qed.
 
 
+(* If an expression is well formed under a given environment, 
+   then all its indices are less than the length of this environment. 
+   Lifting indices more than this length doesn't do anything *)
 Theorem liftX_wfX
- :  forall ix n x tenv
- ,  n = length tenv
- -> wfX tenv x -> liftX ix n x = x.
+ :  forall n d x e
+ ,  d = length e
+ -> wfX e x
+ -> liftX n d x = x.
 Proof.
- intros. gen tenv n.
+ intros. gen e d.
  induction x; intros; simpl; simpl in H0.
  
  Case "XVar".
-  breaka (bge_nat n n0).
+  breaka (bge_nat n0 d).
   apply bge_nat_true in HeqX.
   false. subst. destruct H0.
   eapply get_above_false in H; auto.
@@ -82,46 +126,53 @@ Proof.
 Qed.
 
 
-(* If a term is closed then lifting it doesn't do anything *)
+(* If an expression is closed then it has no free indices. 
+   Lifting it doesn't do anything. *)
 Theorem liftX_closed
- : forall ix x
- , closedX x -> liftX ix 0 x = x.
+ :  forall n x
+ ,  closedX x
+ -> liftX n 0 x = x.
 Proof.
  intros. unfold closedX in H. eapply liftX_wfX; eauto. 
  simpl. auto.
 Qed.
 
 
+(* Substitution of values in values. 
+   Inductively, we need to reason about performing substitutions 
+   at any depth, hence we must prove a property about (subst' d x2 x1) 
+   instead of the weaker (subst x2 x1) that assumes the substitution
+   is taking place at top level.
+ *)
 Theorem subst_value_value_drop
- :  forall ix tenv x1 x2 t1 t2
- ,  get tenv ix = Some t2
- -> closedX x2
- -> TYPE tenv           x1 t1
- -> TYPE (drop ix tenv) x2 t2
- -> TYPE (drop ix tenv) (subst' ix x2 x1) t1.
+ :  forall ix e x1 x2 t1 t2
+ ,  get  e ix = Some t2
+ -> TYPE e           x1 t1
+ -> TYPE (drop ix e) x2 t2
+ -> TYPE (drop ix e) (subst' ix x2 x1) t1.
 Proof.
- intros ix tenv x1 x2 t1 t2. gen ix tenv t1.
- induction x1; intros; simpl; inverts H1.
+ intros ix e x1 x2 t1 t2. gen ix e t1.
+ induction x1; intros; simpl; inverts H0.
 
  Case "XVar".
   fbreak_compare.
-  SCase "n = ix".
-   rewrite liftX_closed; eauto.
-   rewrite H in H5. inverts H5. auto.
+  SCase "i = ix".
+   rewrite H in H4. inverts H4.
+   lets D: type_wfX H1.
 
   SCase "n < ix".
-   apply TYVar. rewrite <- H5. auto.
-   
+   apply TYVar. rewrite <- H4. auto.
+
   SCase "n > ix".
-   apply TYVar. rewrite <- H5.
-   destruct n. 
+   apply TYVar. rewrite <- H4.
+   destruct n.
     false. omega.
     simpl. rewrite nat_minus_zero. apply get_drop_below. omega.
 
  Case "XLam".
   apply TYLam. rewrite drop_rewind.
   apply IHx1; auto.
-  eapply type_check_closed_in_any_tyenv; eauto.
+  eapply type_check_closed_in_any_tyenv; eauto. admit.
 
  Case "XApp".
   eauto.
